@prefix : <http://www.semanticweb.org/vaime/ontologies/2025/2/untitled-ontology-94/> .
@prefix owl: <http://www.w3.org/2002/07/owl#> .
@prefix rdf: <http://www.w3.org/1999/02/22-rdf-syntax-ns#> .
@prefix xml: <http://www.w3.org/XML/1998/namespace> .
@prefix xsd: <http://www.w3.org/2001/XMLSchema#> .
@prefix rdfs: <http://www.w3.org/2000/01/rdf-schema#> .
@base <http://www.semanticweb.org/vaime/ontologies/2025/2/untitled-ontology-94/> .

<http://newVersionMessage> rdf:type owl:Ontology ;
                            owl:imports <https://schema.org/> ;
                            rdfs:comment "This is an ontology for messages developed by VAIMEE. It integrates classes and properties from Schema.org."@en ;
                            owl:versionInfo 1.0 .

#################################################################
#    Object Properties
#################################################################

###  https://onto.vaimee.com/msg#about
<https://onto.vaimee.com/msg#about> rdf:type owl:ObjectProperty ;
                                    rdfs:domain <https://schema.org/CreativeWork> ;
                                    rdfs:range owl:Thing ;
                                    rdfs:comment "The subject matter of the content."@en ;
                                    rdfs:isDefinedBy <https://onto.vaimee.com/msg> ;
                                    rdfs:label "about"@en .


###  https://onto.vaimee.com/msg#hasVariable
<https://onto.vaimee.com/msg#hasVariable> rdf:type owl:ObjectProperty ;
                                          rdfs:domain <https://onto.vaimee.com/msg#Content> ;
                                          rdfs:range <https://onto.vaimee.com/msg#Variable> ;
                                          rdfs:comment "Links a Template or a TemplateContent to individual variables it contains."@en ;
                                          rdfs:isDefinedBy <https://onto.vaimee.com/msg> ;
                                          rdfs:label "has variable"@en .


###  https://onto.vaimee.com/msg#source
<https://onto.vaimee.com/msg#source> rdf:type owl:ObjectProperty ;
                                     rdfs:domain <https://schema.org/CreativeWork> ;
                                     rdfs:range <https://onto.vaimee.com/msg#DACAMBIAREAggregator> ;
                                     rdfs:comment "Indicates the entity responsible for generating the message."@en ;
                                     rdfs:isDefinedBy <https://onto.vaimee.com/msg> ;
                                     rdfs:label "source"@en .


###  https://onto.vaimee.com/msg#toMultipleRecipients
<https://onto.vaimee.com/msg#toMultipleRecipients> rdf:type owl:ObjectProperty ;
                                                   rdfs:subPropertyOf <https://schema.org/toRecipient> ;
                                                   rdfs:domain <https://schema.org/Message> ;
                                                   rdfs:range <https://onto.vaimee.com/msg#NotificationGroup> ;
                                                   rdfs:comment "Specifies that the message is intended for multiple recipients, typically represented by an Audience or group."@en ;
                                                   rdfs:isDefinedBy <https://onto.vaimee.com/msg> ;
                                                   rdfs:label "to multiple recipients"@en .


###  https://onto.vaimee.com/msg#usesTemplate
<https://onto.vaimee.com/msg#usesTemplate> rdf:type owl:ObjectProperty ;
                                           rdfs:domain <https://onto.vaimee.com/msg#TemplateContent> ;
                                           rdfs:range <https://onto.vaimee.com/msg#Template> ;
                                           rdfs:comment "Links an TemplateContent to its corresponding Template. This property indicates that a specific template has been used as the base structure for a personalized message."@en ;
                                           rdfs:isDefinedBy <https://onto.vaimee.com/msg> ;
                                           rdfs:label "uses template"@en .


#################################################################
#    Data properties
#################################################################

###  https://onto.vaimee.com/msg#dateCreated
<https://onto.vaimee.com/msg#dateCreated> rdf:type owl:DatatypeProperty ;
                                          rdfs:domain <https://schema.org/Message> ;
                                          rdfs:range xsd:dateTime ;
                                          rdfs:comment "Specifies the date and time when the message was created."@en ;
                                          rdfs:isDefinedBy <https://onto.vaimee.com/msg> ;
                                          rdfs:label "date created"@en .


###  https://onto.vaimee.com/msg#dateSent
<https://onto.vaimee.com/msg#dateSent> rdf:type owl:DatatypeProperty ;
                                       rdfs:domain <https://schema.org/Message> ;
                                       rdfs:range xsd:dateTime ;
                                       rdfs:comment "Indicates the exact date and time when the message was sent."@en ;
                                       rdfs:isDefinedBy <https://onto.vaimee.com/msg> ;
                                       rdfs:label "date sent"@en .


###  https://onto.vaimee.com/msg#hasValue
<https://onto.vaimee.com/msg#hasValue> rdf:type owl:DatatypeProperty ;
                                       rdfs:domain <https://onto.vaimee.com/msg#Variable> ;
                                       rdfs:range [ rdf:type rdfs:Datatype ;
                                                    owl:unionOf ( xsd:anyURI
                                                                  xsd:boolean
                                                                  xsd:dateTime
                                                                  xsd:dateTimeStamp
                                                                  xsd:decimal
                                                                  xsd:double
                                                                  xsd:float
                                                                  xsd:integer
                                                                  xsd:string
                                                                )
                                                  ] ;
                                       rdfs:comment "Associates a variable with its value."@en ;
                                       rdfs:isDefinedBy <https://onto.vaimee.com/msg> ;
                                       rdfs:label "has value"@en .


###  https://onto.vaimee.com/msg#language
<https://onto.vaimee.com/msg#language> rdf:type owl:DatatypeProperty ;
                                       rdfs:domain <https://onto.vaimee.com/msg#Template> ;
                                       rdfs:range [ rdf:type rdfs:Datatype ;
                                                    owl:unionOf ( xsd:language
                                                                  xsd:string
                                                                )
                                                  ] ;
                                       rdfs:comment "Specifies the language of the template."@en ;
                                       rdfs:isDefinedBy <https://onto.vaimee.com/msg> ;
                                       rdfs:label "langauge"@en .


###  https://onto.vaimee.com/msg#name
<https://onto.vaimee.com/msg#name> rdf:type owl:DatatypeProperty ;
                                   rdfs:domain owl:Thing ;
                                   rdfs:range xsd:string ;
                                   rdfs:comment "Links a resource with its name."@en ;
                                   rdfs:isDefinedBy <https://onto.vaimee.com/msg> ;
                                   rdfs:label "name"@en .


###  https://onto.vaimee.com/msg#text
<https://onto.vaimee.com/msg#text> rdf:type owl:DatatypeProperty ;
                                   rdfs:domain [ rdf:type owl:Class ;
                                                 owl:unionOf ( <https://onto.vaimee.com/msg#Content>
                                                               <https://onto.vaimee.com/msg#Template>
                                                             )
                                               ] ;
                                   rdfs:range xsd:string ;
                                   rdfs:comment "A string of text associated with a resource."@en ;
                                   rdfs:isDefinedBy <https://onto.vaimee.com/msg> ;
                                   rdfs:label "text" .


#################################################################
#    Classes
#################################################################

###  https://onto.vaimee.com/msg#Content
<https://onto.vaimee.com/msg#Content> rdf:type owl:Class ;
                                      rdfs:subClassOf <https://schema.org/CreativeWork> ;
                                      rdfs:comment <https://onto.vaimee.com/msg> ,
                                                   "A generic class representing any kind of content, which can be either a text message or a template message with attachments."@en ;
                                      rdfs:label "Content"@en .


###  https://onto.vaimee.com/msg#DACAMBIAREAggregator
<https://onto.vaimee.com/msg#DACAMBIAREAggregator> rdf:type owl:Class .


###  https://onto.vaimee.com/msg#NotificationGroup
<https://onto.vaimee.com/msg#NotificationGroup> rdf:type owl:Class ;
                                                rdfs:subClassOf <https://schema.org/Audience> ;
                                                rdfs:comment "A collection of recipients grouped together for notification purposes, which may represent a broadcast list, a mailing list, or a messaging group."@en ;
                                                rdfs:isDefinedBy <https://onto.vaimee.com/msg> ;
                                                rdfs:label "Notification Group"@en .


###  https://onto.vaimee.com/msg#Template
<https://onto.vaimee.com/msg#Template> rdf:type owl:Class ;
                                       rdfs:subClassOf <https://schema.org/CreativeWork> ;
                                       rdfs:comment "A text-based template with placeholders for variables."@en ;
                                       rdfs:isDefinedBy <https://onto.vaimee.com/msg> ;
                                       rdfs:label "Template"@en .


###  https://onto.vaimee.com/msg#TemplateContent
<https://onto.vaimee.com/msg#TemplateContent> rdf:type owl:Class ;
                                              rdfs:subClassOf <https://onto.vaimee.com/msg#Content> ;
                                              rdfs:comment "Represents a content that is based on a template, including variables and optional attachments."@en ;
                                              rdfs:isDefinedBy <https://onto.vaimee.com/msg> ;
                                              rdfs:label "Template Content"@en .


###  https://onto.vaimee.com/msg#TextContent
<https://onto.vaimee.com/msg#TextContent> rdf:type owl:Class ;
                                          rdfs:subClassOf <https://onto.vaimee.com/msg#Content> ;
                                          rdfs:comment "Represents a content that is a text message, which can also have attachments."@en ;
                                          rdfs:isDefinedBy <https://onto.vaimee.com/msg> ;
                                          rdfs:label "Text Content"@en .


###  https://onto.vaimee.com/msg#Variable
<https://onto.vaimee.com/msg#Variable> rdf:type owl:Class ;
                                       rdfs:subClassOf <https://schema.org/Intangible> ;
                                       rdfs:comment "A symbolic placeholder representing a value that can be assigned dynamically in different contexts."@en ;
                                       rdfs:isDefinedBy <https://onto.vaimee.com/msg> ;
                                       rdfs:label "Variable"@en .


###  Generated by the OWL API (version 4.5.29.2024-05-13T12:11:03Z) https://github.com/owlcs/owlapi
