@prefix : <http://www.semanticweb.org/vaime/ontologies/2025/2/untitled-ontology-94/> .
@prefix owl: <http://www.w3.org/2002/07/owl#> .
@prefix rdf: <http://www.w3.org/1999/02/22-rdf-syntax-ns#> .
@prefix xml: <http://www.w3.org/XML/1998/namespace> .
@prefix xsd: <http://www.w3.org/2001/XMLSchema#> .
@prefix rdfs: <http://www.w3.org/2000/01/rdf-schema#> .
@base <http://www.semanticweb.org/vaime/ontologies/2025/2/untitled-ontology-94/> .

<http://newVersionMessage> rdf:type owl:Ontology ;
                            owl:imports <https://schema.org/> ;
                            rdfs:comment "This is an ontology for messages developed by VAIMEE. It integrates classes and properties from Schema.org."@en ;
                            owl:versionInfo 1.0 .

#################################################################
#    Object Properties
#################################################################

###  http://newVersionMessage#hasVariable
:hasVariable rdf:type owl:ObjectProperty ;
             rdfs:domain :Content ;
             rdfs:range :Variable ;
             rdfs:comment "Links a Template or a TemplateContent to individual variables it contains."@en ;
             rdfs:isDefinedBy <https://onto.vaimee.com/msg> ;
             rdfs:label "has variable"@en .


###  http://newVersionMessage#usesTemplate
:usesTemplate rdf:type owl:ObjectProperty ;
              rdfs:domain :TemplateContent ;
              rdfs:range :Template ;
              rdfs:comment "Links an TemplateContent to its corresponding Template. This property indicates that a specific template has been used as the base structure for a personalized message."@en ;
              rdfs:isDefinedBy <https://onto.vaimee.com/msg> ;
              rdfs:label "uses template"@en .


###  http://www.semanticweb.org/vaime/ontologies/2025/2/untitled-ontology-94/about
:about rdf:type owl:ObjectProperty ;
       rdfs:domain <https://schema.org/CreativeWork> ;
       rdfs:range owl:Thing ;
       rdfs:comment "The subject matter of the content."@en ;
       rdfs:isDefinedBy <https://onto.vaimee.com/msg> ;
       rdfs:label "about"@en .


###  http://www.semanticweb.org/vaime/ontologies/2025/2/untitled-ontology-94/source
:source rdf:type owl:ObjectProperty ;
        rdfs:domain <https://schema.org/CreativeWork> ;
        rdfs:range :DACAMBIAREAggregator ;
        rdfs:comment "Indicates the entity responsible for generating the message."@en ;
        rdfs:isDefinedBy <https://onto.vaimee.com/msg> ;
        rdfs:label "source"@en .


###  http://www.semanticweb.org/vaime/ontologies/2025/2/untitled-ontology-94/toMultipleRecipients
:toMultipleRecipients rdf:type owl:ObjectProperty ;
                      rdfs:subPropertyOf <https://schema.org/toRecipient> ;
                      rdfs:domain <https://schema.org/Message> ;
                      rdfs:range :NotificationGroup ;
                      rdfs:comment "Specifies that the message is intended for multiple recipients, typically represented by an Audience or group."@en ;
                      rdfs:isDefinedBy <https://onto.vaimee.com/msg> ;
                      rdfs:label "to multiple recipients"@en .


#################################################################
#    Data properties
#################################################################

###  http://newVersionMessage#hasValue
:hasValue rdf:type owl:DatatypeProperty ;
          rdfs:domain :Variable ;
          rdfs:range [ rdf:type rdfs:Datatype ;
                       owl:unionOf ( xsd:anyURI
                                     xsd:boolean
                                     xsd:dateTime
                                     xsd:dateTimeStamp
                                     xsd:decimal
                                     xsd:double
                                     xsd:float
                                     xsd:integer
                                     xsd:string
                                   )
                     ] ;
          rdfs:comment "Associates a variable with its value."@en ;
          rdfs:isDefinedBy <https://onto.vaimee.com/msg> ;
          rdfs:label "has value"@en .


###  http://newVersionMessage#language
:language rdf:type owl:DatatypeProperty ;
          rdfs:domain :Template ;
          rdfs:range [ rdf:type rdfs:Datatype ;
                       owl:unionOf ( xsd:language
                                     xsd:string
                                   )
                     ] ;
          rdfs:comment "Specifies the language of the template."@en ;
          rdfs:isDefinedBy <https://onto.vaimee.com/msg> ;
          rdfs:label "langauge"@en .


###  http://newVersionMessage#name
:name rdf:type owl:DatatypeProperty ;
      rdfs:domain owl:Thing ;
      rdfs:range xsd:string ;
      rdfs:comment "Links a resource with its name."@en ;
      rdfs:isDefinedBy <https://onto.vaimee.com/msg> ;
      rdfs:label "name"@en .


###  http://newVersionMessage#text
:text rdf:type owl:DatatypeProperty ;
      rdfs:domain [ rdf:type owl:Class ;
                    owl:unionOf ( :Content
                                  :Template
                                )
                  ] ;
      rdfs:range xsd:string ;
      rdfs:comment "A string of text associated with a resource."@en ;
      rdfs:isDefinedBy <https://onto.vaimee.com/msg> ;
      rdfs:label "text" .


###  http://www.semanticweb.org/vaime/ontologies/2025/2/untitled-ontology-94/dateCreated
:dateCreated rdf:type owl:DatatypeProperty ;
             rdfs:domain <https://schema.org/Message> ;
             rdfs:range xsd:dateTime ;
             rdfs:comment "Specifies the date and time when the message was created."@en ;
             rdfs:isDefinedBy <https://onto.vaimee.com/msg> ;
             rdfs:label "date created"@en .


###  http://www.semanticweb.org/vaime/ontologies/2025/2/untitled-ontology-94/dateSent
:dateSent rdf:type owl:DatatypeProperty ;
          rdfs:domain <https://schema.org/Message> ;
          rdfs:range xsd:dateTime ;
          rdfs:comment "Indicates the exact date and time when the message was sent."@en ;
          rdfs:isDefinedBy <https://onto.vaimee.com/msg> ;
          rdfs:label "date sent"@en .


#################################################################
#    Classes
#################################################################

###  http://newVersionMessage#Content
:Content rdf:type owl:Class ;
         rdfs:subClassOf <https://schema.org/CreativeWork> ;
         rdfs:comment <https://onto.vaimee.com/msg> ,
                      "A generic class representing any kind of content, which can be either a text message or a template message with attachments."@en ;
         rdfs:label "Content"@en .


###  http://newVersionMessage#NotificationGroup
:NotificationGroup rdf:type owl:Class ;
                   rdfs:subClassOf <https://schema.org/Audience> ;
                   rdfs:comment "A collection of recipients grouped together for notification purposes, which may represent a broadcast list, a mailing list, or a messaging group."@en ;
                   rdfs:isDefinedBy <https://onto.vaimee.com/msg> ;
                   rdfs:label "Notification Group"@en .


###  http://newVersionMessage#Template
:Template rdf:type owl:Class ;
          rdfs:subClassOf <https://schema.org/CreativeWork> ;
          rdfs:comment "A text-based template with placeholders for variables."@en ;
          rdfs:isDefinedBy <https://onto.vaimee.com/msg> ;
          rdfs:label "Template"@en .


###  http://newVersionMessage#TemplateContent
:TemplateContent rdf:type owl:Class ;
                 rdfs:subClassOf :Content ;
                 rdfs:comment "Represents a content that is based on a template, including variables and optional attachments."@en ;
                 rdfs:isDefinedBy <https://onto.vaimee.com/msg> ;
                 rdfs:label "Template Content"@en .


###  http://newVersionMessage#TextContent
:TextContent rdf:type owl:Class ;
             rdfs:subClassOf :Content ;
             rdfs:comment "Represents a content that is a text message, which can also have attachments."@en ;
             rdfs:isDefinedBy <https://onto.vaimee.com/msg> ;
             rdfs:label "Text Content"@en .


###  http://newVersionMessage#Variable
:Variable rdf:type owl:Class ;
          rdfs:subClassOf <https://schema.org/Intangible> ;
          rdfs:comment "A symbolic placeholder representing a value that can be assigned dynamically in different contexts."@en ;
          rdfs:isDefinedBy <https://onto.vaimee.com/msg> ;
          rdfs:label "Variable"@en .


###  http://www.semanticweb.org/vaime/ontologies/2025/2/untitled-ontology-94/DACAMBIAREAggregator
:DACAMBIAREAggregator rdf:type owl:Class .


###  Generated by the OWL API (version 4.5.29.2024-05-13T12:11:03Z) https://github.com/owlcs/owlapi
