@prefix : <https://onto.vaimee.com/jsap#> .
@prefix owl: <http://www.w3.org/2002/07/owl#> .
@prefix rdf: <http://www.w3.org/1999/02/22-rdf-syntax-ns#> .
@prefix xml: <http://www.w3.org/XML/1998/namespace> .
@prefix xsd: <http://www.w3.org/2001/XMLSchema#> .
@prefix rdfs: <http://www.w3.org/2000/01/rdf-schema#> .
@base <https://onto.vaimee.com/jsap#> .

<https://onto.vaimee.com/jsap#> rdf:type owl:Ontology ;
                                 owl:imports <http://xmlns.com/foaf/0.1/> ;
                                 rdfs:comment "This is an ontology for JSAPs developed by VAIMEE. It integrates some classes and properties from FOAF."@en ;
                                 owl:versionInfo 1.0 .

#################################################################
#    Object Properties
#################################################################

###  https://onto.vaimee.com/jsap#hasComponent
:hasComponent rdf:type owl:ObjectProperty ;
              rdfs:domain :JSAP ;
              rdfs:range :PacComponent ;
              owl:propertyChainAxiom ( :includesOperation
                                       [ owl:inverseOf :performsQuery
                                       ]
                                     ) ,
                                     ( :includesOperation
                                       [ owl:inverseOf :performsSubscription
                                       ]
                                     ) ,
                                     ( :includesOperation
                                       [ owl:inverseOf :performsUpdate
                                       ]
                                     ) ;
              rdfs:comment "Inferred link: a JSAP is associated with a PAC component if the component uses an operation defined within the JSAP."@en ;
              rdfs:isDefinedBy <https://onto.vaimee.com/jsap> ;
              rdfs:label "has component"@en .


###  https://onto.vaimee.com/jsap#hasNamespace
:hasNamespace rdf:type owl:ObjectProperty ;
              rdfs:domain :JSAP ;
              rdfs:range :Namespace ;
              rdfs:comment "Links a JSAP instance to a RDF namespace."@en ;
              rdfs:isDefinedBy <https://onto.vaimee.com/jsap> ;
              rdfs:label "has namespace"@en .


###  https://onto.vaimee.com/jsap#includesOperation
:includesOperation rdf:type owl:ObjectProperty ;
                   owl:inverseOf :isOperationOf ;
                   rdfs:domain :JSAP ;
                   rdfs:range :Operation ;
                   rdfs:comment "Associates a JSAP with the operations it contains,"@en ;
                   rdfs:isDefinedBy <https://onto.vaimee.com/jsap> ;
                   rdfs:label "includes operation"@en .


###  https://onto.vaimee.com/jsap#isOperationOf
:isOperationOf rdf:type owl:ObjectProperty ;
               rdfs:domain :Operation ;
               rdfs:range :JSAP ;
               rdfs:comment "Indicates that a given operation is used from a JSAP."@en ;
               rdfs:label <https://onto.vaimee.com/jsap> ,
                          "is operation of"@en .


###  https://onto.vaimee.com/jsap#performsQuery
:performsQuery rdf:type owl:ObjectProperty ;
               rdfs:domain :PacComponent ;
               rdfs:range :Query ;
               rdfs:comment "Declares that the PAC component performs a SPARQL query operation to retrieve data from the knowledge graph."@en ;
               rdfs:isDefinedBy <https://onto.vaimee.com/jsap> ;
               rdfs:label "performs query"@en .


###  https://onto.vaimee.com/jsap#performsSubscription
:performsSubscription rdf:type owl:ObjectProperty ,
                               owl:FunctionalProperty ;
                      rdfs:domain :PacComponent ;
                      rdfs:range :Query ;
                      rdfs:comment "Declares that the PAC component performs a SPARQL subscription operation to continuously monitor changes in the knowledge graph. It is typically used to trigger reactive behavior."@en ;
                      rdfs:isDefinedBy <https://onto.vaimee.com/jsap> ;
                      rdfs:label "performs subscription"@en .


###  https://onto.vaimee.com/jsap#performsUpdate
:performsUpdate rdf:type owl:ObjectProperty ,
                         owl:FunctionalProperty ;
                rdfs:domain :PacComponent ;
                rdfs:range :Update ;
                rdfs:comment "Declares that the PAC component performs a SPARQL update operation that modifies the knowledge graph (e.g., INSERT, DELETE). Each component can make at most one update."@en ;
                rdfs:isDefinedBy <https://onto.vaimee.com/jsap> ;
                rdfs:label "performs update"@en .


###  https://onto.vaimee.com/jsap#usesLiteralFB
:usesLiteralFB rdf:type owl:ObjectProperty ;
               rdfs:domain :Operation ;
               rdfs:range :LiteralFB ;
               rdfs:isDefinedBy <https://onto.vaimee.com/jsap> ;
               rdfs:label "uses literal fb"@en .


###  https://onto.vaimee.com/jsap#usesSnippet
:usesSnippet rdf:type owl:ObjectProperty ;
             rdfs:domain :Operation ;
             rdfs:range :Snippet ;
             rdfs:comment "Indicates that the operation reuses a predefined SPARQL snippet."@en ;
             rdfs:isDefinedBy <https://onto.vaimee.com/jsap> ;
             rdfs:label "uses snippet"@en .


###  https://onto.vaimee.com/jsap#usesUriFB
:usesUriFB rdf:type owl:ObjectProperty ;
           rdfs:domain :Operation ;
           rdfs:range :UriFB ;
           rdfs:comment "Associates the operation with a URI forced binding."@en ;
           rdfs:isDefinedBy <https://onto.vaimee.com/jsap> ;
           rdfs:label "uses URI fb"@en .


#################################################################
#    Data properties
#################################################################

###  https://onto.vaimee.com/jsap#dataValue
:dataValue rdf:type owl:DatatypeProperty ;
           rdfs:domain :LiteralFB ;
           rdfs:comment "The value assigned to the variable in the binding."@en ;
           rdfs:isDefinedBy <https://onto.vaimee.com/jsap> ;
           rdfs:label "dataValue"@en .


###  https://onto.vaimee.com/jsap#name
:name rdf:type owl:DatatypeProperty ;
      rdfs:domain [ rdf:type owl:Class ;
                    owl:unionOf ( :LiteralFB
                                  :UriFB
                                )
                  ] ;
      rdfs:range xsd:string ;
      rdfs:comment "The name of the variable being bound."@en ;
      rdfs:isDefinedBy <https://onto.vaimee.com/jsap> ;
      rdfs:label "name"@en .


###  https://onto.vaimee.com/jsap#prefix
:prefix rdf:type owl:DatatypeProperty ;
        rdfs:domain :Namespace ;
        rdfs:range xsd:string ;
        rdfs:comment "Represents the shorthand prefix used for the namespace (e.g., 'rdf', 'schema')."@en ;
        rdfs:isDefinedBy <https://onto.vaimee.com/jsap> ;
        rdfs:label "prefix"@en .


###  https://onto.vaimee.com/jsap#snippetBody
:snippetBody rdf:type owl:DatatypeProperty ;
             rdfs:domain :Snippet ;
             rdfs:range xsd:string ;
             rdfs:comment "The SPARQL code fragment that can be reused in operations."@en ;
             rdfs:isDefinedBy <https://onto.vaimee.com/jsap> ;
             rdfs:label "snippet body"@en .


###  https://onto.vaimee.com/jsap#sparql
:sparql rdf:type owl:DatatypeProperty ;
        rdfs:domain :Operation ;
        rdfs:range xsd:string ;
        rdfs:comment "The SPARQL query or update string."@en ;
        rdfs:isDefinedBy <https://onto.vaimee.com/jsap> ;
        rdfs:label "sparql"@en .


#################################################################
#    Classes
#################################################################

###  https://onto.vaimee.com/jsap#Aggregator
:Aggregator rdf:type owl:Class ;
            owl:equivalentClass [ owl:intersectionOf ( :PacComponent
                                                       [ rdf:type owl:Restriction ;
                                                         owl:onProperty :performsSubscription ;
                                                         owl:someValuesFrom :Query
                                                       ]
                                                       [ rdf:type owl:Restriction ;
                                                         owl:onProperty :performsUpdate ;
                                                         owl:someValuesFrom :Update
                                                       ]
                                                     ) ;
                                  rdf:type owl:Class
                                ] ;
            rdfs:subClassOf :PacComponent ;
            rdfs:comment "A component of the PAC architecture that processes incoming notifications and triggers an update if necessary. The processing of an aggregator can be combinatorial or sequential."@en ;
            rdfs:isDefinedBy <https://onto.vaimee.com/jsap> ;
            rdfs:label "Aggregator"@en .


###  https://onto.vaimee.com/jsap#Consumer
:Consumer rdf:type owl:Class ;
          owl:equivalentClass [ owl:intersectionOf ( :PacComponent
                                                     [ rdf:type owl:Class ;
                                                       owl:complementOf [ rdf:type owl:Restriction ;
                                                                          owl:onProperty :performsUpdate ;
                                                                          owl:someValuesFrom :Update
                                                                        ]
                                                     ]
                                                     [ rdf:type owl:Restriction ;
                                                       owl:onProperty :performsSubscription ;
                                                       owl:someValuesFrom :Query
                                                     ]
                                                   ) ;
                                rdf:type owl:Class
                              ] ;
          rdfs:subClassOf :PacComponent ;
          rdfs:comment "A component of the PAC architecture that either makes a SPARQL subscription or a SPARQL update, but not both."@en ;
          rdfs:isDefinedBy <https://onto.vaimee.com/jsap> ;
          rdfs:label "Consumer"@en .


###  https://onto.vaimee.com/jsap#ForcedBinding
:ForcedBinding rdf:type owl:Class ;
               rdfs:subClassOf :SPARQLFragment ;
               rdfs:comment "Represents a forced variable binding used in a SPARQL operation within a JSAP."@en ;
               rdfs:isDefinedBy <https://onto.vaimee.com/jsap> ;
               rdfs:label "Forced Binding"@en .


###  https://onto.vaimee.com/jsap#JSAP
:JSAP rdf:type owl:Class ;
      rdfs:comment "Defines a JSAP (JSON SPARQL Application Profile).  JSAP describes an application based on the SPARQL Event Processing Architecture (SEPA) and following the application design pattern named PAC (Producer-Aggregator-Consumer)."@en ;
      rdfs:isDefinedBy <https://onto.vaimee.com/jsap> ;
      rdfs:label "JSAP"@en .


###  https://onto.vaimee.com/jsap#LiteralFB
:LiteralFB rdf:type owl:Class ;
           owl:equivalentClass [ rdf:type owl:Restriction ;
                                 owl:onProperty :dataValue ;
                                 owl:cardinality "1"^^xsd:nonNegativeInteger
                               ] ;
           rdfs:subClassOf :ForcedBinding ;
           owl:disjointWith :UriFB ;
           rdfs:comment "A forced binding whose value is a literal."@en ;
           rdfs:isDefinedBy <https://onto.vaimee.com/jsap> ;
           rdfs:label "Literal FB"@en .


###  https://onto.vaimee.com/jsap#Namespace
:Namespace rdf:type owl:Class ;
           rdfs:comment "Represents an RDF namespace. They allow grouping related terms (classes and properties) under a common base URI."@en ;
           rdfs:isDefinedBy <https://onto.vaimee.com/jsap> ;
           rdfs:label "Namespace"@en .


###  https://onto.vaimee.com/jsap#Operation
:Operation rdf:type owl:Class ;
           rdfs:comment "An abstract superclass representing any operation described in a JSAP."@en ;
           rdfs:isDefinedBy <https://onto.vaimee.com/jsap> ;
           rdfs:label "Operation"@en .


###  https://onto.vaimee.com/jsap#PacComponent
:PacComponent rdf:type owl:Class ;
              rdfs:subClassOf <http://xmlns.com/foaf/0.1/Agent> ;
              rdfs:comment "A component in a JSAP application following the PAC (Producer-Aggregator-Consumer) architectural pattern."@en ;
              rdfs:isDefinedBy <https://onto.vaimee.com/jsap> ;
              rdfs:label "Pac Component"@en .


###  https://onto.vaimee.com/jsap#Producer
:Producer rdf:type owl:Class ;
          owl:equivalentClass [ owl:intersectionOf ( :PacComponent
                                                     [ rdf:type owl:Class ;
                                                       owl:complementOf [ rdf:type owl:Restriction ;
                                                                          owl:onProperty :performsSubscription ;
                                                                          owl:someValuesFrom :Query
                                                                        ]
                                                     ]
                                                     [ rdf:type owl:Restriction ;
                                                       owl:onProperty :performsUpdate ;
                                                       owl:someValuesFrom :Update
                                                     ]
                                                   ) ;
                                rdf:type owl:Class
                              ] ;
          rdfs:subClassOf :PacComponent ;
          rdfs:comment "A component of the PAC architecture that makes exactly one SPARQL update and no subscription."@en ;
          rdfs:isDefinedBy <https://onto.vaimee.com/jsap> ;
          rdfs:label "Producer"@en .


###  https://onto.vaimee.com/jsap#Query
:Query rdf:type owl:Class ;
       rdfs:subClassOf :SPARQLOperation ;
       rdfs:comment "A SPARQL operation that retrieves information from a knowledge base without modifying it. Examples include SELECT, ASK, and CONSTRUCT queries."@en ;
       rdfs:isDefinedBy <https://onto.vaimee.com/jsap> ;
       rdfs:label "Query"@en .


###  https://onto.vaimee.com/jsap#Rule
:Rule rdf:type owl:Class ;
      rdfs:subClassOf :Operation ;
      rdfs:comment "A general-purpose rule defined within a JSAP configuration. A rule can express declarative logic or behavior that triggers specific operations (e.g., updates) under certain conditions."@en ;
      rdfs:isDefinedBy <https://onto.vaimee.com/jsap> ;
      rdfs:label "Rule"@en .


###  https://onto.vaimee.com/jsap#SPARQLFragment
:SPARQLFragment rdf:type owl:Class ;
                rdfs:comment "Defines a fragment of SPARQL that can be inserted into queries or updates, typically through variable substitution or templating mechanisms."@en ;
                rdfs:isDefinedBy <https://onto.vaimee.com/jsap> ;
                rdfs:label "SPARQL Fragment"@en .


###  https://onto.vaimee.com/jsap#SPARQLOperation
:SPARQLOperation rdf:type owl:Class ;
                 rdfs:subClassOf :Operation ;
                 rdfs:comment "Abstract superclass for SPARQL-based operations. It encompasses both queries and updates that interact with the RDF knowledge base using SPARQL 1.1 syntax."@en ;
                 rdfs:isDefinedBy <https://onto.vaimee.com/jsap> ;
                 rdfs:label "SPARQL Operation"@en .


###  https://onto.vaimee.com/jsap#Snippet
:Snippet rdf:type owl:Class ;
         rdfs:subClassOf :SPARQLFragment ;
         rdfs:comment "Represents a reusable SPARQL code fragment that can be included in one or more operations."@en ;
         rdfs:isDefinedBy <https://onto.vaimee.com/jsap> ;
         rdfs:label "Snippet"@en .


###  https://onto.vaimee.com/jsap#Update
:Update rdf:type owl:Class ;
        rdfs:subClassOf :SPARQLOperation ;
        rdfs:comment "A SPARQL operation that modifies the knowledge base by inserting, deleting, or updating triples. Examples include INSERT DATA, DELETE DATA, and DELETE/INSERT operations."@en ;
        rdfs:isDefinedBy <https://onto.vaimee.com/jsap> ;
        rdfs:label "Update"@en .


###  https://onto.vaimee.com/jsap#UriFB
:UriFB rdf:type owl:Class ;
       rdfs:subClassOf :ForcedBinding ;
       rdfs:comment "A URI forced binding: the identifier (URI) of the individual is the value itself."@en ;
       rdfs:isDefinedBy <https://onto.vaimee.com/jsap> ;
       rdfs:label "URI FB"@en .


#################################################################
#    Individuals
#################################################################

###  https://onto.vaimee.com/jsap#agg1
:agg1 rdf:type owl:NamedIndividual ;
      :performsSubscription :q1 .


###  https://onto.vaimee.com/jsap#jsap1
:jsap1 rdf:type owl:NamedIndividual ;
       :includesOperation :q1 .


###  https://onto.vaimee.com/jsap#literalFB
:literalFB rdf:type owl:NamedIndividual ;
           :dataValue 30 .


###  https://onto.vaimee.com/jsap#q1
:q1 rdf:type owl:NamedIndividual .


###  https://onto.vaimee.com/jsap#urifb
:urifb rdf:type owl:NamedIndividual ;
       :name "carlo" .


#################################################################
#    General axioms
#################################################################

[ rdf:type owl:AllDisjointClasses ;
  owl:members ( :Aggregator
                :Consumer
                :Producer
              )
] .


###  Generated by the OWL API (version 4.5.29.2024-05-13T12:11:03Z) https://github.com/owlcs/owlapi
