@prefix : <https://onto.vaimee.com/users#> .
@prefix owl: <http://www.w3.org/2002/07/owl#> .
@prefix rdf: <http://www.w3.org/1999/02/22-rdf-syntax-ns#> .
@prefix xml: <http://www.w3.org/XML/1998/namespace> .
@prefix xsd: <http://www.w3.org/2001/XMLSchema#> .
@prefix rdfs: <http://www.w3.org/2000/01/rdf-schema#> .
@base <https://onto.vaimee.com/users#> .

<https://onto.vaimee.com/users#> rdf:type owl:Ontology ;
                                  owl:imports <https://schema.org/> .

#################################################################
#    Object Properties
#################################################################

###  https://onto.vaimee.com/users#memberOfGroup
:memberOfGroup rdf:type owl:ObjectProperty ;
               rdfs:domain <https://schema.org/ContactPoint> ;
               rdfs:range :NotificationGroup ;
               rdfs:comment "Indicates the association between a contact point and a notification group to which it belongs."@en ;
               rdfs:isDefinedBy <https://onto.vaimee.com/users> ;
               rdfs:label "member of group"@en .


###  https://onto.vaimee.com/users#notificationChannel
:notificationChannel rdf:type owl:ObjectProperty ;
                     rdfs:domain :NotificationPreference ;
                     rdfs:range <https://schema.org/ContactPoint> ;
                     rdfs:comment "Indicates the preferred communication channel through which the user wants to receive notifications about a topic. This can be a ContactPoint such as WhatsApp, Email, or Telegram."@en ;
                     rdfs:isDefinedBy <https://onto.vaimee.com/users> ;
                     rdfs:label "notification channel"@en .


###  https://onto.vaimee.com/users#notificationPreference
:notificationPreference rdf:type owl:ObjectProperty ;
                        rdfs:domain [ rdf:type owl:Class ;
                                      owl:unionOf ( <https://schema.org/Organization>
                                                    <https://schema.org/Person>
                                                  )
                                    ] ;
                        rdfs:range :NotificationPreference ;
                        rdfs:comment "Indicates the notification preferences set by a user or organization. This property links a Person or Organization to their NotificationPreference, which specifies some aspects of the notification, for example: the topic of interest, the preferred communication channels for receiving notifications about this topic and the notification source."@en ;
                        rdfs:isDefinedBy <https://onto.vaimee.com/users> ;
                        rdfs:label "notification preference"@en .


###  https://onto.vaimee.com/users#notificationSource
:notificationSource rdf:type owl:ObjectProperty ;
                    rdfs:domain :NotificationPreference ;
                    rdfs:range :Aggregator ;
                    rdfs:comment "Links a NotificationPreference with the desired source of the notifications."@en ;
                    rdfs:isDefinedBy <https://onto.vaimee.com/users> ;
                    rdfs:label "notification source"@en .


###  https://onto.vaimee.com/users#notificationTopic
:notificationTopic rdf:type owl:ObjectProperty ;
                   rdfs:domain :NotificationPreference ;
                   rdfs:range <https://onto.vaimee.com/users#DACAMBIARE/QUERY> ;
                   rdfs:comment "Defines the topic of interest for which the user wants to receive notifications. This could be the URI of a specific event, category, or query whose result the user wants to receive."@en ;
                   rdfs:isDefinedBy <https://onto.vaimee.com/users> ;
                   rdfs:label "notification topic"@en .


#################################################################
#    Data properties
#################################################################

###  https://onto.vaimee.com/users#identifier
:identifier rdf:type owl:DatatypeProperty ;
            rdfs:domain [ rdf:type owl:Class ;
                          owl:unionOf ( :NotificationGroup
                                        <https://schema.org/ContactPoint>
                                      )
                        ] ;
            rdfs:range [ rdf:type rdfs:Datatype ;
                         owl:unionOf ( xsd:decimal
                                       xsd:integer
                                       xsd:string
                                     )
                       ] ;
            rdfs:comment "This property is used to store the specific identifier of a resource."@en ;
            rdfs:isDefinedBy <https://onto.vaimee.com/users> ;
            rdfs:label "identifier"@en .


#################################################################
#    Classes
#################################################################

###  https://onto.vaimee.com/users#Aggregator
:Aggregator rdf:type owl:Class ;
            rdfs:subClassOf :JsapToCHANGE .


###  https://onto.vaimee.com/users#Channel
:Channel rdf:type owl:Class ;
         rdfs:subClassOf <https://schema.org/ContactPoint> ;
         rdfs:comment "A digital contact point through which a user can receive notifications or communicate."@en ;
         rdfs:isDefinedBy <https://onto.vaimee.com/users> ;
         rdfs:label "Channel"@en .


###  https://onto.vaimee.com/users#Discord
:Discord rdf:type owl:Class ;
         rdfs:subClassOf :Channel ;
         rdfs:comment "A communication channel for voice, text, and video chat within Discord servers."@en ;
         rdfs:isDefinedBy <https://onto.vaimee.com/users> ;
         rdfs:label "Discord"@en .


###  https://onto.vaimee.com/users#Email
:Email rdf:type owl:Class ;
       rdfs:subClassOf :Channel ;
       rdfs:comment "A communication channel based on sending and receiving emails."@en ;
       rdfs:isDefinedBy <https://onto.vaimee.com/users> ;
       rdfs:label "Email"@en .


###  https://onto.vaimee.com/users#JsapToCHANGE
:JsapToCHANGE rdf:type owl:Class .


###  https://onto.vaimee.com/users#NotificationGroup
:NotificationGroup rdf:type owl:Class ;
                   rdfs:subClassOf <https://schema.org/Audience> ;
                   rdfs:comment "A collection of recipients grouped together for notification purposes, which may represent a broadcast list, a mailing list, or a messaging group."@en ;
                   rdfs:isDefinedBy <https://onto.vaimee.com/users> ;
                   rdfs:label "Notification Group"@en .


###  https://onto.vaimee.com/users#NotificationPreference
:NotificationPreference rdf:type owl:Class ;
                        rdfs:subClassOf <https://schema.org/StructuredValue> ,
                                        [ owl:intersectionOf ( [ rdf:type owl:Restriction ;
                                                                 owl:onProperty :notificationChannel ;
                                                                 owl:minQualifiedCardinality "1"^^xsd:nonNegativeInteger ;
                                                                 owl:onClass <https://schema.org/ContactPoint>
                                                               ]
                                                               [ rdf:type owl:Restriction ;
                                                                 owl:onProperty :notificationTopic ;
                                                                 owl:qualifiedCardinality "1"^^xsd:nonNegativeInteger ;
                                                                 owl:onClass <https://onto.vaimee.com/users#DACAMBIARE/QUERY>
                                                               ]
                                                             ) ;
                                          rdf:type owl:Class
                                        ] ;
                        rdfs:comment "Represents a user's or organization's notification preferences. This class defines a topic of interest, the preferred communication channels through which the user wants to receive notifications about that topic and the notification source."@en ;
                        rdfs:isDefinedBy <https://onto.vaimee.com/users> ;
                        rdfs:label "Notification Preference"@en .


###  https://onto.vaimee.com/users#Telegram
:Telegram rdf:type owl:Class ;
          rdfs:subClassOf :Channel ;
          rdfs:comment "A communication channel that uses Telegram for messages, calls, and notifications."@en ;
          rdfs:isDefinedBy <https://onto.vaimee.com/users> ;
          rdfs:label "Telegram"@en .


###  https://onto.vaimee.com/users#WhatsApp
:WhatsApp rdf:type owl:Class ;
          rdfs:subClassOf :Channel ;
          rdfs:comment "A communication channel based on instant messaging via the WhatsApp application."@en ;
          rdfs:isDefinedBy <https://onto.vaimee.com/users> ;
          rdfs:label "WhatsApp"@en .


###  https://onto.vaimee.com/users#DACAMBIARE/QUERY
<https://onto.vaimee.com/users#DACAMBIARE/QUERY> rdf:type owl:Class ;
                                                 rdfs:subClassOf :JsapToCHANGE .


###  Generated by the OWL API (version 4.5.29.2024-05-13T12:11:03Z) https://github.com/owlcs/owlapi
